Avoid names collisions with general bindings file

proof/amd64/avx2/kck_bindings.ec
@@ -1,144 +1,68 @@
 require import AllCore List IntDiv QFABV.
 
 from Jasmin require import JModel_x86.
-
-from CryptoSpecs require export Keccak1600_arrays.
-from JazzEC require import Array7 WArray200 WArray800 Array100.
-
+from JazzEC require import Array4 Array5 Array6 Array7 Array8 Array9 Array16 Array24 Array25 Array32 Array48 Array128 Array160 Array256 Array384 Array768 Array960 Array1088 Array1024 Array1152 Array1408 Array1536 WArray1568 Array1410 Array1 Array2.
+from JazzEC require import WArray16 WArray32 WArray128 WArray160 WArray512 WArray960 WArray2048 WArray1536 Array1568 WArray1410 WArray384 WArray1088.
 
 import BitEncoding BS2Int BitChunking.
 
-(*[size_flatten] (for uniform inner lists) *)
-lemma size_flatten' ['a] sz (ss: 'a list list):
- (forall x, x\in ss => size x = sz) =>
- size (flatten ss) = sz*size ss.
-proof.
-move=> H; rewrite size_flatten.
-rewrite StdBigop.Bigint.sumzE.
-rewrite StdBigop.Bigint.BIA.big_map.
-rewrite -(StdBigop.Bigint.BIA.eq_big_seq (fun _ => sz)) /=.
- by move=> x Hx; rewrite /(\o) /= H.
-by rewrite StdBigop.Bigint.big_constz count_predT.
-qed.
+require import JWord_extra.
 
-lemma flatten_ctt_inj ['a] (n : int) (s s' : 'a list list):
-     0 < n =>
-     (forall (x : 'a list), x \in s => size x = n) =>
-     (forall (x : 'a list), x \in s' => size x = n) =>
-     flatten s = flatten s' <=> s = s'.
-move=> Hn H1 H2; split; last by auto.
-move => Hf.
-have ? : size s = size s'.
-+ have ? := size_flatten_ctt n s _;1:smt().
-  have ? := size_flatten_ctt n s' _;1:smt().
-  have ? : n * size s' = n * size s.
-   have ?: size (flatten s) = size (flatten s') by smt().
-   smt().
-  by smt().
-apply (eq_from_nth []); 1:smt().
-move => i ib.
-apply (eq_from_nth witness);1:smt(mem_nth).
-move => ii iib.
-
-have -> : nth witness (nth [] s i) ii  = nth witness (flatten s) (i * n + ii). rewrite (nth_flatten witness n). rewrite allP => /#. 
- have : 0 <= ii < n. 
-  have n_sz : size (nth [] s i) = n.
-  apply H1.
-   smt(mem_nth).
-  smt(). 
- move => ii_bnd.
- have -> : (i * n + ii) %/ n = i.
-  have -> : (i * n + ii) %/ n = i + (ii %/ n) by rewrite divzMDl /#.
-  smt().
- have -> : (i * n + ii) %% n = ii %% n by rewrite modzMDl /#.
- by rewrite modz_small /#.
-
-have -> : nth witness (nth [] s' i) ii = nth witness (flatten s') (i * n + ii). 
- rewrite (nth_flatten witness n).
-  rewrite allP => /#. 
- have : 0 <= ii < n. 
-  have n_sz : size (nth [] s' i) = n.
-   smt(mem_nth).
-  have : size (nth [] s' i) = size (nth [] s i) by smt(mem_nth).
-  smt().
- move => ii_bnd2.
- have -> : (i * n + ii) %/ n = i.
-  have -> : (i * n + ii) %/ n = i + (ii %/ n) by rewrite divzMDl /#.
-  smt().
- have -> : (i * n + ii) %% n = ii %% n by rewrite modzMDl /#.
- by rewrite modz_small /#.
-
-smt().
-qed.
+require import Kck_abs_bindings.
 
 
-(* ----------- BEGIN BOOL BINDINGS ---------- *)
-op bool2bits (b : bool) : bool list = [b].
-op bits2bool (b: bool list) : bool = List.nth false b 0.
+(* ----------- BEGIN W4 BINDINGS ---------- *)
+theory W4.
+abbrev [-printing] size = 4.
+clone include BitWordSH with op size <- size
+proof gt0_size by done,
+size_le_256 by done.
 
-op i2b (i : int) = (i %% 2 <> 0).
-op b2si (b: bool) = 0.
+end W4. export W4 W4.ALU W4.SHIFT.
 
-bind bitstring bool2bits bits2bool b2i b2si i2b bool 1.
-realize size_tolist by auto.
-realize tolistP by auto.
-realize oflistP by rewrite /bool2bits /bits2bool;smt(size_eq1).
-realize ofintP by rewrite /bits2bool /int2bs => i; rewrite (nth_mkseq false) //. 
-realize touintP by rewrite /bool2bits /= => bv; rewrite bs2int_cons bs2int_nil //=.
-realize tosintP by move => bv => //. 
-realize gt0_size by done.
+clone import JCircuits as JC4 with
+op size <- 4,
+theory W <- W4
+rename "_XX" as "_4".
 
-bind op bool (/\) "and".
-realize bvandP by move=> bv1 bv2; rewrite /bool2bits /#.
+(* ----------- BEGIN W5 BINDINGS ---------- *)
+theory W5.
+abbrev [-printing] size = 5.
+clone include BitWordSH with op size <- size
+proof gt0_size by done,
+size_le_256 by done.
 
-bind op bool (\/) "or".
-realize bvorP by move=> bv1 bv2; rewrite /bool2bits /#.
+end W5. export W5 W5.ALU W5.SHIFT.
 
-bind op bool Bool.(^^) "xor".
-realize bvxorP by move=> bv1 bv2; rewrite /bool2bits /#.
+clone import JCircuits as JC5 with
+op size <- 5,
+theory W <- W5
+rename "_XX" as "_5".
 
-
-(* ------------- BEGIN W8 Bindings -------------------- *)
-
-
+  (* ----------- BEGIN W8 BINDINGS ---------- *)
 bind bitstring W8.w2bits W8.bits2w W8.to_uint W8.to_sint W8.of_int W8.t 8.
 realize size_tolist by auto.
 realize tolistP by auto.
 realize oflistP by smt(W8.bits2wK). 
-realize ofintP by move => *;rewrite /of_int int2bs_mod //=.
-realize tosintP.
- move => bv /=;rewrite /to_sint /smod /BVA_Top_JWord_W8_t.msb.
- have -> /=: nth false (w2bits bv) (8 - 1) = 2 ^ (8 - 1) <= to_uint bv; last by smt().
- rewrite /to_uint -{2}(cat_take_drop 7 (w2bits bv)).
- rewrite bs2int_cat size_take 1:// W8.size_w2bits /=.
- rewrite -bs2int_div 1:// /= get_to_uint /=.
- rewrite -bs2int_mod 1:// /= /to_uint.
- by smt(bs2int_range mem_range W8.size_w2bits pow2_8).
- qed.
+realize ofintP by move => *;rewrite /of_int int2bs_mod.
+realize tosintP. move => bv /=;rewrite /to_sint /smod /BVA_Top_JWord_W8_t.msb.
+have -> /=: nth false (w2bits bv) (8 - 1) = 2 ^ (8 - 1) <= to_uint bv; last by smt().
+rewrite /to_uint. 
+rewrite -{2}(cat_take_drop 7 (w2bits bv)).
+rewrite bs2int_cat size_take 1:// W8.size_w2bits /=.
+rewrite -bs2int_div 1:// /= get_to_uint /=.
+rewrite -bs2int_mod 1:// /= /to_uint.
+by smt(bs2int_range mem_range W8.size_w2bits pow2_8).
+qed.
 realize touintP by smt().
 realize gt0_size by done.
 
 (* -------------------------------------------------------------------- *)
 bind op [W8.t & bool] W8."_.[_]" "get".
+
+realize bvgetP by done.
 realize le_size by done.
 realize eq1_size by done.
-realize bvgetP by done.
-
-(* -------------------------------------------------------------------- *)
-bind op [bool & W8.t] W8.init "init".
-realize size_1 by auto.
-realize bvinitP.
- move=> f; apply (eq_from_nth false).
-  rewrite (size_flatten' 1).
-   move=> x /mkseqP [y [Hy ->]] /=.
-   exact BVA_Top_Pervasive_bool.size_tolist.
-  by rewrite size_w2bits size_mkseq; smt(W8.gt0_size).
- rewrite size_w2bits => i Hi.
- rewrite get_w2bits (BitEncoding.BitChunking.nth_flatten false 1 _).
-  apply/List.allP => x /mkseqP [y [Hy ->]] /=.
-  exact BVA_Top_Pervasive_bool.size_tolist.
- by rewrite (:i %% 1 = 0) 1:/# nth_mkseq 1:/# /bool2bits initiE /=.
- qed.
 
 (* -------------------------------------------------------------------- *)
 bind op W8.t W8.andw "and".
@@ -157,6 +81,7 @@ by rewrite !get_w2bits w2bitsE nth_mkseq //#.
 qed.
 
 bind op W8.t W8.orw "or".
+
 realize bvorP. 
 move => bv1 bv2. 
 apply (eq_from_nth false); 1: by smt(size_map size_zip W8.size_w2bits).
@@ -165,28 +90,9 @@ rewrite (nth_map (false,false) false) /=; 1: by smt(size_map size_zip W8.size_w2
 rewrite !(nth_zip false false) //=;congr; rewrite -W8.get_w2bits.
 qed.
 
-bind op W8.t W8.(+^) "xor".
-realize bvxorP. 
-move => bv1 bv2. 
-apply (eq_from_nth false); 1: by smt(size_map size_zip W8.size_w2bits).
-move => i ib;rewrite !W8.get_w2bits xorwE.
-rewrite (nth_map (false,false) false) /=; 1: by smt(size_map size_zip W8.size_w2bits).  
-rewrite !(nth_zip false false) //=;congr; rewrite -W8.get_w2bits.
-qed.
-
-bind op [W8.t] W8.invw "not".
-realize bvnotP.
-move=> bv1.
-apply (eq_from_nth false); 1: rewrite !size_map size_w2bits /#. 
-move => i; rewrite size_w2bits /= => ib.
-by rewrite (nth_map false) 1:// /= /#.
-qed.
 
 bind op [W8.t & W8.t] W8.(`>>`) "shrs".
-realize bvshrsP.
-rewrite /(`>>`) => bv1 bv2.
-by rewrite W8.to_uint_shr; 1:smt(W8.to_uint_cmp).
-qed.
+realize bvshrsP by move => bv1 bv2; rewrite /(`>>`) to_uint_shr; 1:smt(W8.to_uint_cmp).
 
 op srl_8 (w1 w2 : W8.t) : W8.t =
   w1 `>>>` W8.to_uint w2.
@@ -207,29 +113,164 @@ rewrite /shl_8 => bv1 bv2.
 by rewrite W8.to_uint_shl; 1:smt(W8.to_uint_cmp).
 qed.
 
-(* ------------- END W8 Bindings -------------------- *)
 
-lemma W16_sar_div (w1 : W16.t) k:
- 0 <= k =>
- to_sint (w1 `|>>>` k)
- = to_sint w1 %/ 2 ^ k.
+(* ----------- BEGIN W10 BINDINGS -----------*)
+
+theory W10.
+abbrev [-printing] size = 10.
+clone include BitWordSH with op size <- size
+rename "_XX" as "_10"
+proof gt0_size by done,
+size_le_256 by done.
+
+end W10. export W10 W10.ALU W10.SHIFT.
+
+bind bitstring W10.w2bits W10.bits2w W10.to_uint W10.to_sint W10.of_int W10.t 10.
+realize size_tolist by auto.
+realize tolistP by auto.
+realize oflistP by smt(W10.bits2wK). 
+realize ofintP by move => *;rewrite /of_int int2bs_mod.
+realize tosintP. move => bv /=;rewrite /to_sint /smod /BVA_Top_W10_t.msb.
+have -> /=: nth false (w2bits bv) (10 - 1) = 2 ^ (10 - 1) <= to_uint bv; last by smt().
+rewrite /to_uint. 
+rewrite -{2}(cat_take_drop 9 (w2bits bv)).
+rewrite bs2int_cat size_take 1:// W10.size_w2bits /=.
+rewrite -bs2int_div 1:// /= get_to_uint /=.
+rewrite -bs2int_mod 1:// /= /to_uint.
+have ? : 2^10 = 1024 by rewrite /=.
+by smt(bs2int_range mem_range W10.size_w2bits).
+qed.
+realize touintP by smt().
+realize gt0_size by done.      
+
+bind op [W10.t & bool] W10."_.[_]" "get".
+realize le_size by auto.
+realize eq1_size by auto.
+realize bvgetP by auto.
+
+bind op [bool & W10.t] W10.init "init".
+realize size_1 by auto.
+realize bvinitP.
+move => f.  apply (eq_from_nth false).
++ rewrite size_w2bits (size_flatten' 1). 
+  move => x; rewrite mkseqP /= => Hx;elim Hx.
+  rewrite /bool2bits => /#.
+  rewrite size_mkseq /#.
+
+move => i; rewrite size_w2bits => ?.
+rewrite get_w2bits (nth_flatten false 1).
++ rewrite allP.
+  move => x; rewrite mkseqP /= => Hx;elim Hx.
+  rewrite /bool2bits => /#.
+by rewrite nth_mkseq 1:/# /= /bool2bits initiE 1:/# /=. 
+qed.
+
+(* ----------- BEGIN W10 BINDINGS -----------*)
+
+theory W11.
+abbrev [-printing] size = 11.
+clone include BitWordSH with op size <- size
+rename "_XX" as "_11"
+proof gt0_size by done,
+size_le_256 by done.
+
+end W11. export W11 W11.ALU W11.SHIFT.
+
+bind bitstring W11.w2bits W11.bits2w W11.to_uint W11.to_sint W11.of_int W11.t 11.
+realize size_tolist by auto.
+realize tolistP by auto.
+realize oflistP by smt(W11.bits2wK). 
+realize ofintP by move => *;rewrite /of_int int2bs_mod.
+realize tosintP. move => bv /=;rewrite /to_sint /smod /BVA_Top_W11_t.msb.
+have -> /=: nth false (w2bits bv) (11 - 1) = 2 ^ (11 - 1) <= to_uint bv; last by smt().
+rewrite /to_uint. 
+rewrite -{2}(cat_take_drop 10 (w2bits bv)).
+rewrite bs2int_cat size_take 1:// W11.size_w2bits /=.
+rewrite -bs2int_div 1:// /= get_to_uint /=.
+rewrite -bs2int_mod 1:// /= /to_uint.
+have ? : 2^11 = 2048 by rewrite /=.
+by smt(bs2int_range mem_range W11.size_w2bits).
+qed.
+realize touintP by smt().
+realize gt0_size by done.
+
+
+bind op [W11.t & bool] W11."_.[_]" "get".
+realize le_size by auto.
+realize eq1_size by auto.
+realize bvgetP by auto.
+
+bind op [bool & W11.t] W11.init "init".
+realize size_1 by auto.
+realize bvinitP.
+move => f.  apply (eq_from_nth false).
++ rewrite size_w2bits (size_flatten' 1). 
+  move => x; rewrite mkseqP /= => Hx;elim Hx.
+  rewrite /bool2bits => /#.
+  rewrite size_mkseq /#.
+
+move => i; rewrite size_w2bits => ?.
+rewrite get_w2bits (nth_flatten false 1).
++ rewrite allP.
+  move => x; rewrite mkseqP /= => Hx;elim Hx.
+  rewrite /bool2bits => /#.
+by rewrite nth_mkseq 1:/# /= /bool2bits initiE 1:/# /=. 
+qed.
+
+(* ----------- BEGIN W12 BINDINGS -----------*)
+
+theory W12.
+  abbrev [-printing] size = 12.
+  clone include BitWordSH with op size <- size
+  rename "_XX" as "_12"
+  proof gt0_size by done, size_le_256 by done.
+end W12.
+
+import W12.
+
+(* -------------------------------------------------------------------- *)
+bind bitstring W12.w2bits W12.bits2w W12.to_uint W12.to_sint W12.of_int W12.t 12.
+realize size_tolist by auto.
+realize tolistP     by auto.
+realize oflistP     by smt(W12.bits2wK).
+realize ofintP      by move=> *; rewrite /of_int int2bs_mod.
+realize touintP     by smt().
+
+realize tosintP.
 proof.
-admitted.
+move=> bv /= @/to_sint @/smod @/msb.
+rewrite (_ : nth _ _ _ = 2 ^ (12 - 1) <= to_uint bv) -1:/#.
+rewrite /to_uint -{2}(cat_take_drop 11 (w2bits bv)).
+rewrite bs2int_cat size_take 1:// W12.size_w2bits /=.
+rewrite -bs2int_div 1:// /= get_to_uint /=.
+rewrite -bs2int_mod 1:// /= /to_uint.
+have ?: W12.modulus = 4096 by done.
+by smt(bs2int_range mem_range W12.size_w2bits).
+qed.
+realize gt0_size by done.
 
-lemma W32_sar_div (w1 : W32.t) k:
- 0 <= k =>
- to_sint (w1 `|>>>` k)
- = to_sint w1 %/ 2 ^ k.
-proof.
-admitted.
+bind op [W12.t & bool] W12."_.[_]" "get".
+realize le_size by auto.
+realize eq1_size by auto.
+realize bvgetP by auto.
 
-lemma W64_sar_div (w1 : W64.t) k:
- 0 <= k =>
- to_sint (w1 `|>>>` k)
- = to_sint w1 %/ 2 ^ k.
-proof.
-admitted.
 
+bind op [bool & W12.t] W12.init "init".
+realize size_1 by auto.
+realize bvinitP.
+move => f.  apply (eq_from_nth false).
++ rewrite size_w2bits (size_flatten' 1). 
+  move => x; rewrite mkseqP /= => Hx;elim Hx.
+  rewrite /bool2bits => /#.
+  rewrite size_mkseq /#.
+
+move => i; rewrite size_w2bits => ?.
+rewrite get_w2bits (nth_flatten false 1).
++ rewrite allP.
+  move => x; rewrite mkseqP /= => Hx;elim Hx.
+  rewrite /bool2bits => /#.
+by rewrite nth_mkseq 1:/# /= /bool2bits initiE 1:/# /=.
+qed.
 
 (* ----------- BEGIN W16 BINDINGS ---------- *)
 
@@ -284,23 +325,6 @@ apply (eq_from_nth false);1: rewrite size_map size_zip !size_w2bits /#.
 move => i; rewrite size_w2bits /= => ib.
 rewrite initiE 1:/# (nth_map (false,false)) /=;1: rewrite size_zip !size_w2bits /#. 
 by rewrite !nth_zip /=;1:smt(W16.size_w2bits).
-qed.
-
-bind op W16.t W16.(+^) "xor".
-realize bvxorP. 
-rewrite /map2 => bv1 bv2.
-apply (eq_from_nth false);1: rewrite size_map size_zip !size_w2bits /#. 
-move => i; rewrite size_w2bits /= => ib.
-rewrite (nth_map (false,false)) /=;1: rewrite size_zip !size_w2bits /#. 
-by rewrite !nth_zip /=;1:smt(W16.size_w2bits).
-qed.
-
-bind op [W16.t] W16.invw "not".
-realize bvnotP.
-move=> bv1.
-apply (eq_from_nth false); 1: rewrite !size_map size_w2bits /#. 
-move => i; rewrite size_w2bits /= => ib.
-by rewrite (nth_map false) 1:// /= /#.
 qed.
 
 op W16_sub (a : W16.t, b: W16.t) : W16.t = 
@@ -362,6 +386,40 @@ apply bound_abs; smt(W8.to_uint_cmp pow2_8).
 qed.
 realize le_size by done.
 
+op truncateu12(a : W16.t) : W12.t =
+    W12.of_int (to_uint a).
+
+bind op [W16.t & W12.t] truncateu12 "truncate".
+realize bvtruncateP.
+move => mv; rewrite /truncateu12 /W16.w2bits take_mkseq 1:// /= /w2bits.
+apply (eq_from_nth witness);1: by smt(size_mkseq).
+move => i; rewrite size_mkseq /= /max /= => ib.
+rewrite !nth_mkseq 1..2:// /of_int /to_uint /= get_bits2w 1:// 
+        nth_mkseq 1:// /= get_to_uint 1:// /= /to_uint /=.
+have -> /=: (0 <= i && i < 16) by smt().
+pose a := bs2int (w2bits mv). 
+rewrite {1}(divz_eq a (2^(12-i)*2^i)) !mulrA divzMDl;
+   1: by smt(StdOrder.IntOrder.expr_gt0).
+rewrite dvdz_modzDl; 1: by
+ have ->  : 2^(12-i) = 2^((12-i-1)+1); [ by smt() |
+    rewrite exprS 1:/#; smt(dvdz_mull dvdz_mulr)].  
+by have -> : (2 ^ (12 - i) * 2 ^ i) = 4096; 
+  [ rewrite -StdBigop.Bigint.Num.Domain.exprD_nneg 
+     1,2:/# /= -!addrA /= | done ].
+qed.
+realize le_size by done.
+
+op zeroextu16(a : W12.t) : W16.t =
+    W16.of_int (to_uint a).
+
+bind op [W12.t & W16.t] zeroextu16 "zextend".
+realize bvzextendP.
+move => bv; rewrite /zeroextu16 /= of_uintK /=.
+have /= := W12.to_uint_cmp.
+by smt().
+qed.
+realize le_size by done.
+
 bind op [bool & W16.t] W16.init "init".
 realize size_1 by auto.
 realize bvinitP.
@@ -378,6 +436,9 @@ rewrite get_w2bits (nth_flatten false 1).
   rewrite /bool2bits => /#.
 by rewrite nth_mkseq 1:/# /= /bool2bits initiE 1:/# /=. 
 qed.
+
+
+
 
 (* ----------- BEGIN W32 BINDINGS ---------- *)
 
@@ -428,23 +489,6 @@ apply (eq_from_nth false);1: rewrite size_map size_zip !size_w2bits /#.
 move => i; rewrite size_w2bits /= => ib.
 rewrite initiE 1:/# (nth_map (false,false)) /=;1: rewrite size_zip !size_w2bits /#. 
 by rewrite !nth_zip /=;1:smt(W32.size_w2bits).
-qed.
-
-bind op W32.t W32.(+^) "xor".
-realize bvxorP. 
-rewrite /xorw /map2 => bv1 bv2.
-apply (eq_from_nth false);1: rewrite size_map size_zip !size_w2bits /#. 
-move => i; rewrite size_w2bits /= => ib.
-rewrite (nth_map (false,false)) /=;1: rewrite size_zip !size_w2bits /#. 
-by rewrite !nth_zip /=;1:smt(W32.size_w2bits).
-qed.
-
-bind op [W32.t] W32.invw "not".
-realize bvnotP.
-move=> bv1.
-apply (eq_from_nth false); 1: rewrite !size_map size_w2bits /#. 
-move => i; rewrite size_w2bits /= => ib.
-by rewrite (nth_map false) 1:// /= /#.
 qed.
 
 op sll_32 (w1 w2 : W32.t) : W32.t =
@@ -530,6 +574,87 @@ by have -> : (2 ^ (16 - i) * 2 ^ i) = 65536;
      1,2:/# /= -!addrA /= | done ].
 qed.
 realize le_size by done.
+
+op truncateu32_4(a : W32.t) : W4.t =
+    W4.of_int (to_uint a).
+
+bind op [W32.t & W4.t] truncateu32_4 "truncate".
+realize bvtruncateP.
+move => mv; rewrite /truncateu32_4 /W32.w2bits take_mkseq 1:// /= /w2bits.
+apply (eq_from_nth witness);1: by smt(size_mkseq).
+move => i; rewrite size_mkseq /= /max /= => ib.
+rewrite !nth_mkseq 1..2:// /of_int /to_uint /= get_bits2w 1:// 
+        nth_mkseq 1:// /= get_to_uint 1:// /= /to_uint /=.
+have -> /=: (0 <= i && i < 32) by smt().
+pose a := bs2int (w2bits mv). 
+rewrite {1}(divz_eq a (2^(4-i)*2^i)) !mulrA divzMDl;
+   1: by smt(StdOrder.IntOrder.expr_gt0).
+rewrite dvdz_modzDl; 1: by
+ have ->  : 2^(4-i) = 2^((4-i-1)+1); [ by smt() |
+    rewrite exprS 1:/#; smt(dvdz_mull dvdz_mulr)].  
+by have -> : (2 ^ (4 - i) * 2 ^ i) = 16; 
+  [ rewrite -StdBigop.Bigint.Num.Domain.exprD_nneg 
+     1,2:/# /= -!addrA /= | done ].
+qed.
+realize le_size by done.
+
+op zeroextu4_32(a : W4.t) : W32.t =
+  W32.of_int (to_uint a).
+
+bind op [W4.t & W32.t] zeroextu4_32 "zextend".
+realize bvzextendP by move => bv; rewrite /zeroextu4_32 /= of_uintK /=; smt(W4.to_uint_cmp pow2_4).
+realize le_size by done.
+
+op truncateu32_5(a : W32.t) : W5.t =
+    W5.of_int (to_uint a).
+
+bind op [W32.t & W5.t] truncateu32_5 "truncate".
+realize bvtruncateP.
+move => mv; rewrite /truncateu32_5 /W32.w2bits take_mkseq 1:// /= /w2bits.
+apply (eq_from_nth witness);1: by smt(size_mkseq).
+move => i; rewrite size_mkseq /= /max /= => ib.
+rewrite !nth_mkseq 1..2:// /of_int /to_uint /= get_bits2w 1:// 
+        nth_mkseq 1:// /= get_to_uint 1:// /= /to_uint /=.
+have -> /=: (0 <= i && i < 32) by smt().
+pose a := bs2int (w2bits mv). 
+rewrite {1}(divz_eq a (2^(5-i)*2^i)) !mulrA divzMDl;
+   1: by smt(StdOrder.IntOrder.expr_gt0).
+rewrite dvdz_modzDl; 1: by
+ have ->  : 2^(5-i) = 2^((5-i-1)+1); [ by smt() |
+    rewrite exprS 1:/#; smt(dvdz_mull dvdz_mulr)].  
+by have -> : (2 ^ (5 - i) * 2 ^ i) = 32; 
+  [ rewrite -StdBigop.Bigint.Num.Domain.exprD_nneg 
+     1,2:/# /= -!addrA /= | done ].
+qed.
+realize le_size by done.
+
+op zeroextu5_32(a : W5.t) : W32.t =
+  W32.of_int (to_uint a).
+
+bind op [W5.t & W32.t] zeroextu5_32 "zextend".
+realize bvzextendP by move => bv; rewrite /zeroextu5_32 /= of_uintK /=; smt(W5.to_uint_cmp pow2_5).
+realize le_size by done.
+
+op zeroextu10_32(a : W10.t) : W32.t =
+  W32.of_int (to_uint a).
+
+bind op [W10.t & W32.t] zeroextu10_32 "zextend".
+realize bvzextendP.
+have ? : 2^10 = 1024 by auto.
+ by move => bv; rewrite /zeroextu32 /= of_uintK /=; smt(W10.to_uint_cmp).
+qed.
+realize le_size by done.
+
+op zeroextu11_32(a : W11.t) : W32.t =
+  W32.of_int (to_uint a).
+
+bind op [W11.t & W32.t] zeroextu11_32 "zextend".
+realize bvzextendP.
+have ? : 2^11 = 2048 by auto.
+ by move => bv; rewrite /zeroextu32 /= of_uintK /=; smt(W11.to_uint_cmp).
+qed.
+realize le_size by done.
+
 
 bind op [W32.t & bool] W32."_.[_]" "get".
 realize bvgetP by rewrite /bool2bits.
@@ -635,6 +760,7 @@ move => i; rewrite size_w2bits /= => ib.
 by rewrite (nth_map false) 1:// /= /#.
 qed.
 
+
 op srl_64 (w1 w2 : W64.t) : W64.t =
   w1 `>>>` to_uint w2.
 
@@ -697,6 +823,50 @@ by have -> : (2 ^ (16 - i) * 2 ^ i) = 65536;
 qed.
 realize le_size by done.
 
+op truncate64_10 (bw: W64.t) : W10.t = W10.of_int (W64.to_uint bw).
+
+bind op [W64.t & W10.t] truncate64_10 "truncate".
+realize bvtruncateP. 
+move => mv; rewrite /truncate64_10 /W64.w2bits take_mkseq 1:// /= /w2bits.
+apply (eq_from_nth witness);1: by smt(size_mkseq).
+move => i; rewrite size_mkseq /= /max /= => ib.
+rewrite !nth_mkseq 1..2:// /of_int /to_uint /= get_bits2w 1:// 
+        nth_mkseq 1:// /= get_to_uint 1:// /= /to_uint /=.
+have -> /=: (0 <= i && i < 64) by smt().
+pose a := bs2int (w2bits mv). 
+rewrite {1}(divz_eq a (2^(10-i)*2^i)) !mulrA divzMDl;
+   1: by smt(StdOrder.IntOrder.expr_gt0).
+rewrite dvdz_modzDl; 1: by
+ have ->  : 2^(10-i) = 2^((10-i-1)+1); [ by smt() |
+    rewrite exprS 1:/#; smt(dvdz_mull dvdz_mulr)].  
+by have -> : (2 ^ (10 - i) * 2 ^ i) = 1024; 
+  [ rewrite -StdBigop.Bigint.Num.Domain.exprD_nneg 
+     1,2:/# /= -!addrA /= | done ].
+qed.
+realize le_size by done.
+
+op truncate64_11 (bw: W64.t) : W11.t = W11.of_int (W64.to_uint bw).
+
+bind op [W64.t & W11.t] truncate64_11 "truncate".
+realize bvtruncateP. 
+move => mv; rewrite /truncate64_11 /W64.w2bits take_mkseq 1:// /= /w2bits.
+apply (eq_from_nth witness);1: by smt(size_mkseq).
+move => i; rewrite size_mkseq /= /max /= => ib.
+rewrite !nth_mkseq 1..2:// /of_int /to_uint /= get_bits2w 1:// 
+        nth_mkseq 1:// /= get_to_uint 1:// /= /to_uint /=.
+have -> /=: (0 <= i && i < 64) by smt().
+pose a := bs2int (w2bits mv). 
+rewrite {1}(divz_eq a (2^(11-i)*2^i)) !mulrA divzMDl;
+   1: by smt(StdOrder.IntOrder.expr_gt0).
+rewrite dvdz_modzDl; 1: by
+ have ->  : 2^(11-i) = 2^((11-i-1)+1); [ by smt() |
+    rewrite exprS 1:/#; smt(dvdz_mull dvdz_mulr)].  
+by have -> : (2 ^ (11 - i) * 2 ^ i) = 2048; 
+  [ rewrite -StdBigop.Bigint.Num.Domain.exprD_nneg 
+     1,2:/# /= -!addrA /= | done ].
+qed.
+realize le_size by done.
+
 bind op [W64.t & W8.t] W8u8.truncateu8 "truncate".
 realize bvtruncateP.  (* generalize *)
 move => mv; rewrite /truncateu8 /W64.w2bits take_mkseq 1:// /= /w2bits.
@@ -737,61 +907,6 @@ by smt(bs2int_range mem_range W128.size_w2bits pow2_128).
 qed.
 realize touintP by smt().
 realize gt0_size by done.
-
-bind op [bool & W128.t] W128.init "init".
-realize bvinitP.
-move=> f; apply (eq_from_nth false).
- rewrite (size_flatten' 1).
-  move=> x /mkseqP [y [Hy ->]] /=.
-  exact BVA_Top_Pervasive_bool.size_tolist.
- by rewrite size_w2bits size_mkseq /#.
-rewrite size_w2bits => i Hi.
-rewrite get_w2bits (BitEncoding.BitChunking.nth_flatten false 1 _).
- apply/List.allP => x /mkseqP [y [Hy ->]] /=.
- exact BVA_Top_Pervasive_bool.size_tolist.
-by rewrite (:i %% 1 = 0) 1:/# nth_mkseq 1:/# /bool2bits initiE /=.
-qed.
-realize size_1 by done.
-
-bind op [W128.t & bool] W128."_.[_]" "get".
-realize bvgetP by rewrite /bool2bits.
-realize le_size by done.
-realize eq1_size by done.
-
-bind op W128.t W128.andw "and".
-realize bvandP. 
-rewrite /andw /map2 => bv1 bv2.
-apply (eq_from_nth false);1: rewrite size_map size_zip !size_w2bits /#. 
-move => i; rewrite size_w2bits /= => ib.
-rewrite initiE 1:/# (nth_map (false,false)) /=;1: rewrite size_zip !size_w2bits /#. 
-by rewrite !nth_zip /=;1:smt(W64.size_w2bits).
-qed.
-
-bind op W128.t W128.orw "or".
-realize bvorP. 
-rewrite /orw /map2 => bv1 bv2.
-apply (eq_from_nth false);1: rewrite size_map size_zip !size_w2bits /#. 
-move => i; rewrite size_w2bits /= => ib.
-rewrite initiE 1:/# (nth_map (false,false)) /=;1: rewrite size_zip !size_w2bits /#. 
-by rewrite !nth_zip /=;1:smt(W64.size_w2bits).
-qed.
-
-bind op [W128.t] W128.(+^) "xor".
-realize bvxorP.
-move => bv1 bv2.
-apply (eq_from_nth false); 1: rewrite !size_map size_zip !size_w2bits /#. 
-move => i; rewrite size_w2bits /= => ib.
-rewrite (nth_map (false,false)) /=; 1: rewrite size_zip !size_w2bits /#. 
-by rewrite !nth_zip /=; 1:smt(W64.size_w2bits).
-qed.
-
-bind op [W128.t] W128.invw "not".
-realize bvnotP.
-move=> bv1.
-apply (eq_from_nth false); 1: rewrite !size_map size_w2bits /#. 
-move => i; rewrite size_w2bits /= => ib.
-by rewrite (nth_map false) 1:// /= /#.
-qed.
 
 bind op [W64.t & W128.t] W2u64.zeroextu128 "zextend".
 realize bvzextendP by move => bv; rewrite /zeroextu128 /= of_uintK /=; smt(W64.to_uint_cmp pow2_64).
@@ -911,9 +1026,6 @@ move => i; rewrite size_w2bits /= => ib.
 by rewrite (nth_map false) 1:// /= /#.
 qed.
 
-bind op [W128.t & W256.t] W2u128.zeroextu256 "zextend".
-realize bvzextendP by move => bv; rewrite /zeroextu256 /= of_uintK /=; smt(W128.to_uint_cmp pow2_128).
-realize le_size by done.
 
 bind op [W256.t & W128.t] W2u128.truncateu128 "truncate".
 realize bvtruncateP.
@@ -938,12 +1050,396 @@ realize le_size by done.
 
 (* ----------- BEGIN ARRAY BINDINGS ---------- *)
 
+bind array Array256."_.[_]" Array256."_.[_<-_]" Array256.to_list Array256.of_list Array256.t 256.
+realize tolistP by done.
+realize get_setP by smt(Array256.get_setE). 
+realize eqP by smt(Array256.tP).
+realize get_out by smt(Array256.get_out).
+realize gt0_size by done.
+
+bind array Array384."_.[_]" Array384."_.[_<-_]" Array384.to_list Array384.of_list Array384.t 384.
+realize tolistP by done.
+realize get_setP by smt(Array384.get_setE). 
+realize eqP by smt(Array384.tP).
+realize get_out by smt(Array384.get_out).
+realize gt0_size by done.
+
+bind array Array768."_.[_]" Array768."_.[_<-_]" Array768.to_list Array768.of_list Array768.t 768.
+realize tolistP by done.
+realize get_setP by smt(Array768.get_setE). 
+realize eqP by smt(Array768.tP).
+realize get_out by smt(Array768.get_out).
+realize gt0_size by done.
+
+bind array Array1024."_.[_]" Array1024."_.[_<-_]" Array1024.to_list Array1024.of_list Array1024.t 1024.
+realize tolistP by done.
+realize get_setP by smt(Array1024.get_setE). 
+realize eqP by smt(Array1024.tP).
+realize get_out by smt(Array1024.get_out).
+realize gt0_size by done.
+
+bind array Array1088."_.[_]" Array1088."_.[_<-_]" Array1088.to_list Array1088.of_list Array1088.t 1088.
+realize tolistP by done.
+realize get_setP by smt(Array1088.get_setE). 
+realize eqP by smt(Array1088.tP).
+realize get_out by smt(Array1088.get_out).
+realize gt0_size by done.
+
+bind array Array1152."_.[_]" Array1152."_.[_<-_]" Array1152.to_list Array1152.of_list Array1152.t 1152.
+realize tolistP by done.
+realize get_setP by smt(Array1152.get_setE). 
+realize eqP by smt(Array1152.tP).
+realize get_out by smt(Array1152.get_out).
+realize gt0_size by done.
+
+bind array Array1408."_.[_]" Array1408."_.[_<-_]" Array1408.to_list Array1408.of_list Array1408.t 1408.
+realize tolistP by done.
+realize get_setP by smt(Array1408.get_setE). 
+realize eqP by smt(Array1408.tP).
+realize get_out by smt(Array1408.get_out).
+realize gt0_size by done.
+
+bind array Array1536."_.[_]" Array1536."_.[_<-_]" Array1536.to_list Array1536.of_list Array1536.t 1536.
+realize tolistP by done.
+realize get_setP by smt(Array1536.get_setE). 
+realize eqP by smt(Array1536.tP).
+realize get_out by smt(Array1536.get_out).
+realize gt0_size by done.
+
+bind array Array1568."_.[_]" Array1568."_.[_<-_]" Array1568.to_list Array1568.of_list Array1568.t 1568.
+realize tolistP by done.
+realize get_setP by smt(Array1568.get_setE). 
+realize eqP by smt(Array1568.tP).
+realize get_out by smt(Array1568.get_out).
+realize gt0_size by done.
+
+bind array Array32."_.[_]" Array32."_.[_<-_]" Array32.to_list Array32.of_list Array32.t 32.
+realize tolistP by done.
+realize get_setP by smt(Array32.get_setE). 
+realize eqP by smt(Array32.tP).
+realize get_out by smt(Array32.get_out).
+realize gt0_size by done.
+
+bind array Array16."_.[_]" Array16."_.[_<-_]" Array16.to_list Array16.of_list Array16.t 16.
+realize tolistP by done.
+realize get_setP by smt(Array16.get_setE). 
+realize eqP by smt(Array16.tP).
+realize get_out by smt(Array16.get_out).
+realize gt0_size by done.
+
+bind array Array48."_.[_]" Array48."_.[_<-_]" Array48.to_list Array48.of_list Array48.t 48.
+realize tolistP by done.
+realize get_setP by smt(Array48.get_setE). 
+realize eqP by smt(Array48.tP).
+realize get_out by smt(Array48.get_out).
+realize gt0_size by done.
+
+bind array Array128."_.[_]" Array128."_.[_<-_]" Array128.to_list Array128.of_list Array128.t 128.
+realize tolistP by done.
+realize get_setP by smt(Array128.get_setE). 
+realize eqP by smt(Array128.tP).
+realize get_out by smt(Array128.get_out).
+realize gt0_size by done.
+
+bind array Array160."_.[_]" Array160."_.[_<-_]" Array160.to_list Array160.of_list Array160.t 160.
+realize tolistP by done.
+realize get_setP by smt(Array160.get_setE). 
+realize eqP by smt(Array160.tP).
+realize get_out by smt(Array160.get_out).
+realize gt0_size by done.
+
+bind array Array960."_.[_]" Array960."_.[_<-_]" Array960.to_list Array960.of_list Array960.t 960.
+realize tolistP by done.
+realize get_setP by smt(Array960.get_setE). 
+realize eqP by smt(Array960.tP).
+realize get_out by smt(Array960.get_out).
+realize gt0_size by done.
+
+bind array Array1410."_.[_]" Array1410."_.[_<-_]" Array1410.to_list Array1410.of_list Array1410.t 1410.
+realize tolistP by done.
+realize get_setP by smt(Array1410.get_setE). 
+realize eqP by smt(Array1410.tP).
+realize get_out by smt(Array1410.get_out).
+realize gt0_size by done.
+
+bind array Array4."_.[_]" Array4."_.[_<-_]" Array4.to_list Array4.of_list Array4.t 4.
+realize tolistP by done.
+realize get_setP by smt(Array4.get_setE). 
+realize eqP by smt(Array4.tP).
+realize get_out by smt(Array4.get_out).
+realize gt0_size by done.
+
+bind array Array1."_.[_]" Array1."_.[_<-_]" Array1.to_list Array1.of_list Array1.t 1.
+realize tolistP by done.
+realize get_setP by smt(Array1.get_setE). 
+realize eqP by smt(Array1.tP).
+realize get_out by smt(Array1.get_out).
+realize gt0_size by done.
+
+bind array Array2."_.[_]" Array2."_.[_<-_]" Array2.to_list Array2.of_list Array2.t 2.
+realize tolistP by done.
+realize get_setP by smt(Array2.get_setE). 
+realize eqP by smt(Array2.tP).
+realize get_out by smt(Array2.get_out).
+realize gt0_size by done.
+
 bind array Array5."_.[_]" Array5."_.[_<-_]" Array5.to_list Array5.of_list Array5.t 5.
 realize tolistP by done.
 realize get_setP by smt(Array5.get_setE). 
 realize eqP by smt(Array5.tP).
 realize get_out by smt(Array5.get_out).
 realize gt0_size by done.
+
+bind array Array6."_.[_]" Array6."_.[_<-_]" Array6.to_list Array6.of_list Array6.t 6.
+realize tolistP by done.
+realize get_setP by smt(Array6.get_setE). 
+realize eqP by smt(Array6.tP).
+realize get_out by smt(Array6.get_out).
+realize gt0_size by done.
+
+bind array Array7."_.[_]" Array7."_.[_<-_]" Array7.to_list Array7.of_list Array7.t 7.
+realize tolistP by done.
+realize get_setP by smt(Array7.get_setE). 
+realize eqP by smt(Array7.tP).
+realize get_out by smt(Array7.get_out).
+realize gt0_size by done.
+
+bind array Array8."_.[_]" Array8."_.[_<-_]" Array8.to_list Array8.of_list Array8.t 8.
+realize tolistP by done.
+realize get_setP by smt(Array8.get_setE). 
+realize eqP by smt(Array8.tP).
+realize get_out by smt(Array8.get_out).
+realize gt0_size by done.
+
+bind array Array24."_.[_]" Array24."_.[_<-_]" Array24.to_list Array24.of_list Array24.t 24.
+realize tolistP by done.
+realize get_setP by smt(Array24.get_setE). 
+realize eqP by smt(Array24.tP).
+realize get_out by smt(Array24.get_out).
+realize gt0_size by done.
+
+bind array Array25."_.[_]" Array25."_.[_<-_]" Array25.to_list Array25.of_list Array25.t 25.
+realize tolistP by done.
+realize get_setP by smt(Array25.get_setE). 
+realize eqP by smt(Array25.tP).
+realize get_out by smt(Array25.get_out).
+realize gt0_size by done.
+
+op init_array16_w16(f : int -> W16.t) = Array16.init f.
+bind op [W16.t & Array16.t] init_array16_w16 "ainit".
+realize bvainitP.
+proof.
+rewrite /init_array16_w16 => f.
+rewrite BVA_Top_Array16_Array16_t.tolistP.
+apply eq_in_mkseq => i i_bnd;
+smt(Array16.initE).
+qed.
+
+op init_array24_w8(f : int -> W8.t) = Array24.init f.
+bind op [W8.t & Array24.t] init_array24_w8 "ainit".
+realize bvainitP.
+rewrite /init_array26_w8 => f.
+rewrite BVA_Top_Array24_Array24_t.tolistP.
+apply eq_in_mkseq => i i_bnd;
+smt(Array24.initE).
+qed.
+
+op init_array32_w16(f : int -> W16.t) = Array32.init f.
+bind op [W16.t & Array32.t] init_array32_w16 "ainit".
+realize bvainitP.
+rewrite /init_array32_w16 => f.
+rewrite BVA_Top_Array32_Array32_t.tolistP.
+apply eq_in_mkseq => i i_bnd;
+smt(Array32.initE).
+qed.
+
+op init_array48_w8(f : int -> W8.t) = Array48.init f.
+bind op [W8.t & Array48.t] init_array48_w8 "ainit".
+realize bvainitP.
+rewrite /init_array48_w8 => f.
+rewrite BVA_Top_Array48_Array48_t.tolistP.
+apply eq_in_mkseq => i i_bnd;
+smt(Array48.initE).
+qed.
+
+op init_32_8 (f: int -> W8.t) : W8.t Array32.t = Array32.init f.
+
+bind op [W8.t & Array32.t] init_32_8 "ainit".
+realize bvainitP.
+proof.
+rewrite /init_32_8 => f.
+rewrite BVA_Top_Array32_Array32_t.tolistP.
+apply eq_in_mkseq => i i_bnd;
+smt(Array32.initE).
+qed.
+
+op init_1088_8(f : int -> W8.t) = Array1088.init f.
+bind op [W8.t & Array1088.t] init_1088_8 "ainit".
+realize bvainitP.
+rewrite /init_1088_8 => f.
+rewrite BVA_Top_Array1088_Array1088_t.tolistP.
+apply eq_in_mkseq => i i_bnd;
+smt(Array1088.initE).
+qed.
+
+op init_768_10(f : int -> W10.t) = Array768.init f.
+bind op [W10.t & Array768.t] init_768_10 "ainit".
+realize bvainitP.
+rewrite /init_768_10 => f.
+rewrite BVA_Top_Array768_Array768_t.tolistP.
+apply eq_in_mkseq => i i_bnd;
+smt(Array768.initE).
+qed.
+
+op init_1568_8 (f: int -> W8.t) : W8.t Array1568.t = Array1568.init f.
+
+bind op [W8.t & Array1568.t] init_1568_8 "ainit".
+realize bvainitP.
+proof.
+rewrite /init_1568_8 => f.
+rewrite BVA_Top_Array1568_Array1568_t.tolistP.
+apply eq_in_mkseq => i i_bnd;
+smt(Array1568.initE).
+qed.
+
+op init_1536_8 (f: int -> W8.t) : W8.t Array1536.t = Array1536.init f.
+
+bind op [W8.t & Array1536.t] init_1536_8 "ainit".
+realize bvainitP.
+proof.
+rewrite /init_1536_8 => f.
+rewrite BVA_Top_Array1536_Array1536_t.tolistP.
+apply eq_in_mkseq => i i_bnd;
+smt(Array1536.initE).
+qed.
+
+op init_1024_8 (f: int -> W8.t) : W8.t Array1024.t = Array1024.init f.
+
+bind op [W8.t & Array1024.t] init_1024_8 "ainit".
+realize bvainitP.
+proof.
+rewrite /init_1024_8 => f.
+rewrite BVA_Top_Array1024_Array1024_t.tolistP.
+apply eq_in_mkseq => i i_bnd;
+smt(Array1024.initE).
+qed.
+
+op init_8_8 (f: int -> W8.t) : W8.t Array8.t = Array8.init f.
+
+bind op [W8.t & Array8.t] init_8_8 "ainit".
+realize bvainitP.
+proof.
+rewrite /init_8_8 => f.
+rewrite BVA_Top_Array8_Array8_t.tolistP.
+apply eq_in_mkseq => i i_bnd;
+smt(Array8.initE).
+qed.
+
+op init_8_16 (f: int -> W16.t) : W16.t Array8.t = Array8.init f.
+
+bind op [W16.t & Array8.t] init_8_16 "ainit".
+realize bvainitP.
+proof.
+rewrite /init_8_16 => f.
+rewrite BVA_Top_Array8_Array8_t.tolistP.
+apply eq_in_mkseq => i i_bnd;
+smt(Array8.initE).
+qed.
+
+op init_160_8 (f: int -> W8.t) : W8.t Array160.t = Array160.init f.
+
+bind op [W8.t & Array160.t] init_160_8 "ainit".
+realize bvainitP.
+proof.
+rewrite /init_160_8 => f.
+rewrite BVA_Top_Array160_Array160_t.tolistP.
+apply eq_in_mkseq => i i_bnd;
+smt(Array160.initE).
+qed.
+
+op init_1152_8 (f: int -> W8.t) : W8.t Array1152.t = Array1152.init f.
+
+bind op [W8.t & Array1152.t] init_1152_8 "ainit".
+realize bvainitP.
+proof.
+rewrite /init_1152_8 => f.
+rewrite BVA_Top_Array1152_Array1152_t.tolistP.
+apply eq_in_mkseq => i i_bnd;
+smt(Array1152.initE).
+qed.
+
+op init_128_8 (f: int -> W8.t) : W8.t Array128.t = Array128.init f.
+
+bind op [W8.t & Array128.t] init_128_8 "ainit".
+realize bvainitP.
+proof.
+rewrite /init_128_8 => f.
+rewrite BVA_Top_Array128_Array128_t.tolistP.
+apply eq_in_mkseq => i i_bnd;
+smt(Array128.initE).
+qed.
+
+op init_384_8 (f: int -> W8.t) : W8.t Array384.t = Array384.init f.
+
+bind op [W8.t & Array384.t] init_384_8 "ainit".
+realize bvainitP.
+proof.
+rewrite /init_384_8 => f.
+rewrite BVA_Top_Array384_Array384_t.tolistP.
+apply eq_in_mkseq => i i_bnd;
+smt(Array384.initE).
+qed.
+
+op init_256_16 (f: int -> W16.t) : W16.t Array256.t = Array256.init f.
+
+bind op [W16.t & Array256.t] init_256_16 "ainit".
+realize bvainitP.
+proof.
+rewrite /init_256_16 => f.
+rewrite BVA_Top_Array256_Array256_t.tolistP.
+apply eq_in_mkseq => i i_bnd;
+smt(Array256.initE).
+qed.
+
+op init_768_16 (f: int -> W16.t) : W16.t Array768.t = Array768.init f.
+
+bind op [W16.t & Array768.t] init_768_16 "ainit".
+realize bvainitP.
+rewrite /init_768_16 => f.
+rewrite BVA_Top_Array768_Array768_t.tolistP.
+apply eq_in_mkseq => i i_bnd; smt(Array768.initE).
+qed.
+
+op init_1024_16 (f: int -> W16.t) : W16.t Array1024.t = Array1024.init f.
+
+bind op [W16.t & Array1024.t] init_1024_16 "ainit".
+realize bvainitP.
+rewrite /init_1024_16 => f.
+rewrite BVA_Top_Array1024_Array1024_t.tolistP.
+apply eq_in_mkseq => i i_bnd; smt(Array1024.initE).
+qed.
+
+op init_4_64 (f: int -> W64.t) : W64.t Array4.t = Array4.init f.
+
+bind op [W64.t & Array4.t] init_4_64 "ainit".
+realize bvainitP.
+proof.
+rewrite /init_4_64 => f.
+rewrite BVA_Top_Array4_Array4_t.tolistP.
+apply eq_in_mkseq => i i_bnd; smt(Array4.initE).
+qed.
+
+op init_5_32 (f: int -> W32.t) : W32.t Array5.t = Array5.init f.
+
+bind op [W32.t & Array5.t] init_5_32 "ainit".
+realize bvainitP.
+proof.
+rewrite /init_5_32 => f.
+rewrite BVA_Top_Array5_Array5_t.tolistP.
+apply eq_in_mkseq => i i_bnd; smt(Array5.initE).
+qed.
+
+op init_5_64 (f: int -> W64.t) = Array5.init f.
 
 bind op [W64.t & Array5.t] init_5_64 "ainit".
 realize bvainitP.
@@ -954,58 +1450,19 @@ apply eq_in_mkseq => i i_bnd;
 smt(Array5.initE).
 qed.
 
-bind array Array25."_.[_]" Array25."_.[_<-_]" Array25.to_list Array25.of_list Array25.t 25.
-realize gt0_size by done.
-realize tolistP by done.
-realize get_setP by smt(Array25.get_setE). 
-realize eqP by smt(Array25.tP).
-realize get_out by smt(Array25.get_out).
+op init_6_256 (f: int -> W256.t) = Array6.init f.
 
-bind op [W64.t & Array25.t] init_25_64 "ainit".
+bind op [W256.t & Array6.t] init_6_256 "ainit".
 realize bvainitP.
 proof.
-rewrite /init_25_64 => f.
-rewrite BVA_Top_Array25_Array25_t.tolistP.
+rewrite /init_6_256 => f.
+rewrite BVA_Top_Array6_Array6_t.tolistP.
 apply eq_in_mkseq => i i_bnd;
-smt(Array25.initE).
+smt(Array6.initE).
 qed.
 
-op init_25_256 = Array25.init <:W256.t>.
-bind op [W256.t & Array25.t] init_25_256 "ainit".
-realize bvainitP.
-proof.
-rewrite /init_25_256 => f.
-rewrite BVA_Top_Array25_Array25_t.tolistP.
-apply eq_in_mkseq => i i_bnd;
-smt(Array25.initE).
-qed.
+op init_7_256 (f: int -> W256.t) = Array7.init f.
 
-
-
-bind array Array24."_.[_]" Array24."_.[_<-_]" Array24.to_list Array24.of_list Array24.t 24.
-realize tolistP by done.
-realize get_setP by smt(Array24.get_setE). 
-realize eqP by smt(Array24.tP).
-realize get_out by smt(Array24.get_out).
-realize gt0_size by done.
-
-bind op [W64.t & Array24.t] init_24_64 "ainit".
-realize bvainitP.
-proof.
-rewrite /init_24_64 => f.
-rewrite BVA_Top_Array24_Array24_t.tolistP.
-apply eq_in_mkseq => i i_bnd;
-smt(Array24.initE).
-qed.
-
-bind array Array7."_.[_]" Array7."_.[_<-_]" Array7.to_list Array7.of_list Array7.t 7.
-realize tolistP by done.
-realize get_setP by smt(Array7.get_setE). 
-realize eqP by smt(Array7.tP).
-realize get_out by smt(Array7.get_out).
-realize gt0_size by done.
-
-op init_7_256 = Array7.init <:W256.t>.
 bind op [W256.t & Array7.t] init_7_256 "ainit".
 realize bvainitP.
 proof.
@@ -1015,199 +1472,80 @@ apply eq_in_mkseq => i i_bnd;
 smt(Array7.initE).
 qed.
 
+op init_25_64 (f: int -> W64.t) = Array25.init f.
 
-bind array Array100."_.[_]" Array100."_.[_<-_]" Array100.to_list Array100.of_list Array100.t 100.
-realize gt0_size by done.
-realize tolistP by done.
-realize get_setP by smt(Array100.get_setE). 
-realize eqP by smt(Array100.tP).
-realize get_out by smt(Array100.get_out).
-    
-op init_100_64 = Array100.init <:W64.t>.
-bind op [W64.t & Array100.t] init_100_64 "ainit".
+bind op [W64.t & Array25.t] init_25_64 "ainit".
 realize bvainitP.
 proof.
-rewrite /init_100_64 => f.
-rewrite BVA_Top_Array100_Array100_t.tolistP.
+rewrite /init_25_64 => f.
+rewrite BVA_Top_Array25_Array25_t.tolistP.
+by apply eq_in_mkseq => i i_bnd; smt(Array25.initE).
+qed.
+
+op init_960_8 (f: int -> W8.t) : W8.t Array960.t = Array960.init f.
+
+bind op [W8.t & Array960.t] init_960_8 "ainit".
+realize bvainitP.
+proof.
+rewrite /init_960_8 => f.
+rewrite BVA_Top_Array960_Array960_t.tolistP.
+apply eq_in_mkseq => i i_bnd; smt(Array960.initE).
+qed.
+
+op init_1408_8 (f: int -> W8.t) : W8.t Array1408.t = Array1408.init f.
+
+bind op [W8.t & Array1408.t] init_1408_8 "ainit".
+realize bvainitP.
+proof.
+rewrite /init_1408_8 => f.
+rewrite BVA_Top_Array1408_Array1408_t.tolistP.
+apply eq_in_mkseq => i i_bnd; smt(Array1408.initE).
+qed.
+
+op init_256_12 (f: int -> W12.t) : W12.t Array256.t = 
+  Array256.init f.
+
+bind op [W12.t & Array256.t] init_256_12 "ainit".
+realize bvainitP.
+rewrite /init_256_12 => f.
+rewrite BVA_Top_Array256_Array256_t.tolistP.
 apply eq_in_mkseq => i i_bnd;
-smt(Array100.initE).
+smt(Array256.initE).
+qed.
+
+op init_1024_12 (f: int -> W12.t) : W12.t Array1024.t = 
+  Array1024.init f.
+
+bind op [W12.t & Array1024.t] init_1024_12 "ainit".
+realize bvainitP.
+rewrite /init_1024_12 => f.
+rewrite BVA_Top_Array1024_Array1024_t.tolistP.
+apply eq_in_mkseq => i i_bnd;
+smt(Array1024.initE).
 qed.
 
 
-op sliceget256_64_100 (arr: W64.t Array100.t) (offset:int): W256.t =
- if 8 %| offset
- then WArray800.get256_direct
-       (WArray800.init64 (fun i => arr.[i]))
-       (offset %/ 8)
- else W256.bits2w (take 256 (drop offset (flatten (map W64.w2bits (to_list arr))))).
+op init_768_12 (f: int -> W12.t) : W12.t Array768.t = 
+  Array768.init f.
 
-bind op [W64.t & W256.t & Array100.t] sliceget256_64_100 "asliceget".
-realize le_size by done.       
-realize bvaslicegetP.
-move => /= arr offset; rewrite /sliceget256_64_100 /= => H k kb. 
-case (8 %| offset) => /= *; last by smt(W256.get_bits2w).
-rewrite /get256_direct pack32E initiE 1:/# /= initiE 1:/# /= initiE 1:/# /= bits8E initiE 1:/# /=.
-rewrite nth_take 1,2:/# nth_drop 1,2:/#.
-rewrite (BitEncoding.BitChunking.nth_flatten false 64 _). 
- by rewrite allP => x /=; rewrite mapP => He; elim He;smt(W64.size_w2bits).
-rewrite (nth_map W64.zero []); 1: smt(Array100.size_to_list).
-by rewrite nth_mkseq /#.
+bind op [W12.t & Array768.t] init_768_12 "ainit".
+realize bvainitP.
+rewrite /init_768_12 => f.
+rewrite BVA_Top_Array768_Array768_t.tolistP.
+apply eq_in_mkseq => i i_bnd;
+smt(Array768.initE).
 qed.
 
-op sliceget64_256_25 (arr: W256.t Array25.t) (offset:int): W64.t =
- if 8 %| offset
- then WArray800.get64_direct
-       (WArray800.init256 (fun i => arr.[i]))
-       (offset %/ 8)
- else W64.bits2w (take 64 (drop offset (flatten (map W256.w2bits (to_list arr))))).
+op init_1024_11 (f: int -> W11.t) : W11.t Array1024.t = Array1024.init f.
 
-bind op [W256.t & W64.t & Array25.t] sliceget64_256_25 "asliceget".
-realize le_size by done.       
-realize bvaslicegetP.
-move => /= arr offset; rewrite /sliceget64_256_25 /= => H k kb. 
-case (8 %| offset) => /= *; last by smt(W64.get_bits2w).
-rewrite /get64_direct pack8E initiE 1:/# /= initiE 1:/# /= initiE 1:/# /= bits8E initiE 1:/# /=.
-rewrite nth_take 1,2:/# nth_drop 1,2:/#.
-rewrite (BitEncoding.BitChunking.nth_flatten false 256 _). 
- by rewrite allP => x /=; rewrite mapP => He; elim He;smt(W256.size_w2bits).
-rewrite (nth_map W256.zero []); 1: smt(Array25.size_to_list).
-by rewrite nth_mkseq /#.
+bind op [W11.t & Array1024.t] init_1024_11 "ainit".
+realize bvainitP.
+rewrite /init_1024_11 => f.
+rewrite BVA_Top_Array1024_Array1024_t.tolistP.
+apply eq_in_mkseq => i i_bnd;
+smt(Array1024.initE).
 qed.
 
-op sliceset64_256_25 (arr: W256.t Array25.t) (offset: int) (bv: W64.t) : W256.t Array25.t =
- if 8 %| offset
- then Array25.init 
-       (fun i =>
-        WArray800.get256
-         (WArray800.set64_direct
-           (WArray800.init256 (fun j => arr.[j]))
-           (offset %/ 8)
-           bv)
-         i)
- else Array25.of_list
-       witness
-       (map W256.bits2w
-            (chunk 256
-                   (take offset (flatten (map W256.w2bits (to_list arr)))
-                     ++ w2bits bv ++
-                     drop (offset+64) (flatten (map W256.w2bits (to_list arr)))))).
-
-lemma size_flatten_W256_w2bits (a : W256.t list) :
-  (size (flatten (map W256.w2bits (a))))  =  256 * size a.
-proof.
-rewrite (size_flatten' 256).
- by move=> l /mapP [x [Hx ->]]; rewrite W256.size_w2bits.
-by rewrite size_map.
-qed.
-
-bind op [W256.t & W64.t & Array25.t] sliceset64_256_25 "asliceset".
-realize le_size by done.
-realize bvaslicesetP.
-move => arr offset bv H /= k kb; rewrite /sliceset64_256_25 /=.
-case (8 %| offset) => /= *; last first.
-+ rewrite of_listK; 1: by rewrite size_map size_chunk 1:// !size_cat size_take;
-      by smt(size_take size_drop  W256.size_w2bits size_cat Array25.size_to_list size_flatten_W256_w2bits size_ge0). 
-  rewrite -(map_comp W256.w2bits W256.bits2w) /(\o). 
-  have := eq_in_map ((fun (x : bool list) => w2bits ((bits2w x))%W256)) idfun (chunk 256
-        (take offset (flatten (map W256.w2bits (to_list arr))) ++ w2bits bv ++
-         drop (offset + 64) (flatten (map W256.w2bits (to_list arr))))).
-  rewrite iffE => [#] -> * /=; 1: by smt(in_chunk_size W256.bits2wK).
-  rewrite map_id /= chunkK 1://;1: by rewrite !size_cat size_take;
-    by smt(size_take size_drop  W256.size_w2bits size_cat Array25.size_to_list size_flatten_W256_w2bits size_ge0). 
-  by rewrite !nth_cat !size_cat /=;
-     smt(nth_take nth_drop size_take size_drop  W256.size_w2bits size_cat Array25.size_to_list size_flatten_W256_w2bits size_ge0). 
-rewrite (nth_flatten _ 256); 1: by rewrite allP => i;rewrite mapP => He; elim He;smt(W256.size_w2bits).
-rewrite (nth_map W256.zero []); 1: smt(Array25.size_to_list).
-rewrite nth_mkseq 1:/# /= initiE 1:/# /= get256E pack32E initiE 1:/# /= initiE 1:/# /= /set64_direct.
-rewrite initiE 1:/# /=.
-case (offset <= k && k < offset + 64) => *; 1: by 
-  rewrite ifT 1:/#  get_bits8 /= 1,2:/# initiE // initiE //.
-rewrite ifF 1:/# initiE 1:/# /=.
-rewrite (nth_flatten _ 256); 1: by rewrite allP => i;rewrite mapP => He; elim He;smt(W256.size_w2bits).
-rewrite (nth_map W256.zero []); 1: smt(Array25.size_to_list).
-rewrite nth_mkseq 1:/# /= bits8E /= initiE /# /=.
-qed.
-
-
-op sliceget256_64_25 (arr: W64.t Array25.t) (offset:int): W256.t =
- if 8 %| offset
- then WArray200.get256_direct
-       (WArray200.init64 (fun i => arr.[i]))
-       (offset %/ 8)
- else W256.bits2w (take 256 (drop offset (flatten (map W64.w2bits (to_list arr))))).
-
-bind op [W64.t & W256.t & Array25.t] sliceget256_64_25 "asliceget".
-realize le_size by done.
-realize bvaslicegetP.
-move => /= arr offset; rewrite /sliceget256_64_25 /= => H k kb. 
-case (8 %| offset) => /= *; last by smt(W256.get_bits2w).
-rewrite /get256_direct pack32E initiE 1:/# /= initiE 1:/# /= initiE 1:/# /= bits8E initiE 1:/# /=.
-rewrite nth_take 1,2:/# nth_drop 1,2:/#.
-rewrite (BitEncoding.BitChunking.nth_flatten false 64 _). 
- by rewrite allP => x /=; rewrite mapP => He; elim He;smt(W64.size_w2bits).
-rewrite (nth_map W64.zero []); 1: smt(Array25.size_to_list).
-by rewrite nth_mkseq /#.
-qed.
-
-op sliceset256_64_25 (arr: W64.t Array25.t) (offset: int) (bv: W256.t) : W64.t Array25.t =
- if 8 %| offset
- then Array25.init 
-       (fun i =>
-        WArray200.get64
-         (WArray200.set256_direct
-           (WArray200.init64 (fun j => arr.[j]))
-           (offset %/ 8)
-           bv)
-         i)
- else Array25.of_list
-       witness
-       (map W64.bits2w
-            (chunk 64
-                   (take offset (flatten (map W64.w2bits (to_list arr)))
-                     ++ w2bits bv ++
-                     drop (offset+256) (flatten (map W64.w2bits (to_list arr)))))).
-
-lemma size_flatten_W64_w2bits (a : W64.t list) :
-  (size (flatten (map W64.w2bits (a))))  =  64 * size a.
-proof.
-rewrite (size_flatten' 64).
- by move=> l /mapP [x [Hx ->]]; rewrite W64.size_w2bits.
-by rewrite size_map.
-qed.
-
-bind op [W64.t & W256.t & Array25.t] sliceset256_64_25 "asliceset".
-realize le_size by done.
-realize bvaslicesetP. 
-move => arr offset bv H /= k kb; rewrite /sliceset256_64_25 /=.
-case (8 %| offset) => /= *; last first.
-+ rewrite of_listK; 1: by rewrite size_map size_chunk 1:// !size_cat size_take;
-      by smt(size_take size_drop  W64.size_w2bits size_cat Array25.size_to_list size_flatten_W64_w2bits size_ge0). 
-  rewrite -(map_comp W64.w2bits W64.bits2w) /(\o). 
-  have := eq_in_map ((fun (x : bool list) => w2bits ((bits2w x))%W64)) idfun (chunk 64
-        (take offset (flatten (map W64.w2bits (to_list arr))) ++ w2bits bv ++
-         drop (offset + 256) (flatten (map W64.w2bits (to_list arr))))).
-  rewrite iffE => [#] -> * /=; 1: by smt(in_chunk_size W64.bits2wK).
-  rewrite map_id /= chunkK 1://;1: by rewrite !size_cat size_take;
-    by smt(size_take size_drop  W64.size_w2bits size_cat Array25.size_to_list size_flatten_W64_w2bits size_ge0). 
-  by rewrite !nth_cat !size_cat /=;
-     smt(nth_take nth_drop size_take size_drop  W64.size_w2bits size_cat Array25.size_to_list size_flatten_W64_w2bits size_ge0). 
-rewrite (nth_flatten _ 64); 1: by rewrite allP => i;rewrite mapP => He; elim He;smt(W64.size_w2bits).
-rewrite (nth_map W64.zero []); 1: smt(Array25.size_to_list).
-rewrite nth_mkseq 1:/# /= initiE 1:/# /= get64E pack8E initiE 1:/# /= initiE 1:/# /= /set256_direct.
-rewrite initiE 1:/# /=.
-case (offset <= k && k < offset + 256) => *; 1: by 
-  rewrite ifT 1:/#  get_bits8 /= 1,2:/# initiE // initiE //.
-rewrite ifF 1:/# initiE 1:/# /=.
-rewrite (nth_flatten _ 64); 1: by rewrite allP => i;rewrite mapP => He; elim He;smt(W64.size_w2bits).
-rewrite (nth_map W64.zero []); 1: smt(Array25.size_to_list).
-rewrite nth_mkseq 1:/# /= bits8E /= initiE /# /=.
-qed.
-
-
-
-
-
-(*
 op sliceget8_32_256 (arr: W32.t Array8.t) (offset: int) : W256.t = 
    if 8 %| offset then 
     get256_direct ((init32 (fun (i_0 : int) => arr.[i_0])))%WArray32 (offset %/ 8)
@@ -1950,14 +2288,11 @@ rewrite BVA_Top_Array4_Array4_t.tolistP.
 apply eq_in_mkseq => i i_bnd;
 smt(Array4.initE).
 qed.
-*)
+
+
 
 (* BEGIN BIND CIRCUITS *)
 bind circuit
-    VMOVLPD <- "VMOVLPD",
-    VMOVHPD <- "VMOVHPD",
-    VMOV_64 <- "VMOV_64",
-    VPINSR_2u64 <- "VPINSR_2u64",
     VPBROADCAST_16u16 <- "VPBROADCAST_16u16",
     VPBROADCAST_8u32 <- "VPBROADCAST_8u32",
     VPBROADCAST_4u64 <- "VPBROADCAST_4u64",
@@ -1965,7 +2300,7 @@ bind circuit
     VPSLLV_8u32 <- "VPSLLV_8u32",
     VPSHUFB_256 <- "VPSHUFB_256",
     VEXTRACTI128 <- "VEXTRACTI128",
-    VINSERTI128  <- "VPINSERTI128",
+    VINSERTI128    <-   "VPINSERTI128",
     VPBLENDW_128 <- "VPBLENDW_128",
     BLENDV_16u8 <- "VPBLENDVB_128",
     VPEXTR_32 <- "VEXTRACTI32_256",
@@ -2011,5 +2346,6 @@ bind circuit
     VPCMPGT_16u16  <-   "VPCMPGT_16u16",
     VPACKSS_16u16  <-   "VPACKSS_16u16"
 
-    from "avx2.spec".
+    from "../common/avx2.spec".
+
 
